deps/poulet4/lib/Relations.v
@@ -13,8 +13,80 @@ Definition rel_true: forall {A}, relation A :=
 Notation "⊤" := rel_true.
 Notation "x ⊓ y" := (relation_conjunction x y) (at level 40).
 
-Fixpoint interp_rels {A} (R: rels A) : relation A :=
-  match R with
-  | [] => ⊤
-  | r :: R' => r ⊓ interp_rels R'
-  end.
+Definition interp_rels {A} (R: rels A) : relation A :=
+  List.fold_right relation_conjunction ⊤ R.
+
+Notation "⟦ R ⟧" := (interp_rels R).
+
+Local Program Instance f_Equivalence {A B} {equiv: rel B} `{Equivalence B equiv} (f: A -> B): Equivalence (fun x y => equiv (f x) (f y)).
+Next Obligation.
+  repeat intro.
+  eapply Equivalence_Reflexive; eauto.
+Qed.
+Next Obligation.
+  repeat intro.
+  eapply Equivalence_Symmetric; eauto.
+Qed.
+Next Obligation.
+  repeat intro.
+  eapply Equivalence_Transitive; eauto.
+Qed.
+
+Definition rels_equiv {A} (R S: rels A) : Prop :=
+  relation_equivalence ⟦R⟧ ⟦S⟧.
+
+Global Program Instance rels_Equivalence {A}: Equivalence (@rels_equiv A) :=
+  ltac:(typeclasses eauto).
+
+Lemma interp_rels_in:
+  forall A (R: rels A),
+    forall x y,
+      interp_rels R x y ->
+      forall r, In r R -> r x y.
+Proof.
+  induction R; intros.
+  - inversion H0.
+  - inversion H0; subst; clear H0.
+    + simpl in *.
+      apply H.
+    + destruct H; eapply IHR; auto.
+Qed.
+
+Lemma in_interp_rels:
+  forall A (R: rels A),
+    forall x y,
+    (forall r, In r R -> r x y) ->
+    interp_rels R x y.
+Proof.
+  induction R; intros.
+  - exact I.
+  - simpl; split.
+    + apply H.
+      eauto with datatypes. 
+    + apply IHR; intros.
+      eapply H.
+      right.
+      apply H0.
+Qed.
+
+Lemma interp_rels_mono:
+  forall A (R S: rels A),
+    forall x y,
+      interp_rels S x y ->
+      (forall r, In r R -> In r S) ->
+      interp_rels R x y.
+Proof.
+  induction R.
+  - intros.
+    exact I.
+  - unfold interp_rels in *.
+    intros.
+    simpl.
+    split.
+    + assert (In a (a :: R))
+        by (eauto with datatypes).
+      eapply interp_rels_in in H; eauto.
+    + eapply (IHR S); eauto.
+      intros.
+      eauto with datatypes.
+Qed.
